Make internals of `coPset` local.

stdpp/coPset.v
@@ -36,56 +36,58 @@ Local Open Scope positive_scope.
 
 (** [coPLeaf false] is the empty set; [coPLeaf true] is the full set. *)
 (** In [coPNode b l r], the Boolean flag [b] indicates whether the number
-    1 is a member of the set, while the subtrees [l] and [r] must be
-    consulted to determine whether a number of the form [2i] or [2i+1]
-    is a member of the set. *)
+1 is a member of the set, while the subtrees [l] and [r] must be
+consulted to determine whether a number of the form [2i] or [2i+1]
+is a member of the set. *)
+(** This [Inductive] is internal, but Rocq does not allow us to make it
+[Local]. *)
 Inductive coPset_raw :=
   | coPLeaf : bool → coPset_raw
   | coPNode : bool → coPset_raw → coPset_raw → coPset_raw.
-Global Instance coPset_raw_eq_dec : EqDecision coPset_raw.
+Local Instance coPset_raw_eq_dec : EqDecision coPset_raw.
 Proof. solve_decision. Defined.
 
 (** The type of raw trees (above) offers several representations of the
-    empty set and several representations of the full set. In order to
-    achieve extensional equality, this redundancy must be eliminated.
-    This is achieved by imposing a well-formedness criterion on trees. *)
-
-Fixpoint coPset_wf (t : coPset_raw) : bool :=
+empty set and several representations of the full set. In order to
+achieve extensional equality, this redundancy must be eliminated.
+This is achieved by imposing a well-formedness criterion on trees. *)
+Local Fixpoint coPset_wf (t : coPset_raw) : bool :=
   match t with
   | coPLeaf _ => true
   | coPNode true (coPLeaf true) (coPLeaf true) => false
   | coPNode false (coPLeaf false) (coPLeaf false) => false
   | coPNode _ l r => coPset_wf l && coPset_wf r
   end.
-Global Arguments coPset_wf !_ / : simpl nomatch, assert.
+Local Arguments coPset_wf !_ / : simpl nomatch, assert.
 
-Lemma coPNode_wf b l r :
+Local Lemma coPNode_wf b l r :
   coPset_wf l → coPset_wf r →
   (l = coPLeaf true → r = coPLeaf true → b = true → False) →
   (l = coPLeaf false → r = coPLeaf false → b = false → False) →
   coPset_wf (coPNode b l r).
 Proof. destruct b, l as [[]|], r as [[]|]; naive_solver. Qed.
 
-Lemma coPNode_wf_l b l r : coPset_wf (coPNode b l r) → coPset_wf l.
+Local Lemma coPNode_wf_l b l r : coPset_wf (coPNode b l r) → coPset_wf l.
 Proof. destruct b, l as [[]|],r as [[]|]; simpl; rewrite ?andb_True; tauto. Qed.
-Lemma coPNode_wf_r b l r : coPset_wf (coPNode b l r) → coPset_wf r.
+Local Lemma coPNode_wf_r b l r : coPset_wf (coPNode b l r) → coPset_wf r.
 Proof. destruct b, l as [[]|],r as [[]|]; simpl; rewrite ?andb_True; tauto. Qed.
 Local Hint Immediate coPNode_wf_l coPNode_wf_r : core.
 
 (** The smart constructor [coPNode'] preserves well-formedness. *)
-Definition coPNode' (b : bool) (l r : coPset_raw) : coPset_raw :=
+Local Definition coPNode' (b : bool) (l r : coPset_raw) : coPset_raw :=
   match b, l, r with
   | true, coPLeaf true, coPLeaf true => coPLeaf true
   | false, coPLeaf false, coPLeaf false => coPLeaf false
   | _, _, _ => coPNode b l r
   end.
-Global Arguments coPNode' : simpl never.
-Lemma coPNode'_wf b l r : coPset_wf l → coPset_wf r → coPset_wf (coPNode' b l r).
+Local Arguments coPNode' : simpl never.
+Local Lemma coPNode'_wf b l r :
+  coPset_wf l → coPset_wf r → coPset_wf (coPNode' b l r).
 Proof. destruct b, l as [[]|], r as [[]|]; simpl; auto. Qed.
-Global Hint Resolve coPNode'_wf : core.
+Local Hint Resolve coPNode'_wf : core.
 
 (** The membership test. *)
-Fixpoint coPset_elem_of_raw (p : positive) (t : coPset_raw) {struct t} : bool :=
+Local Fixpoint coPset_elem_of_raw (p : positive) (t : coPset_raw) {struct t} : bool :=
   match t, p with
   | coPLeaf b, _ => b
   | coPNode b l r, 1 => b
@@ -93,13 +95,13 @@ Fixpoint coPset_elem_of_raw (p : positive) (t : coPset_raw) {struct t} : bool :=
   | coPNode _ _ r, p~1 => coPset_elem_of_raw p r
   end.
 Local Notation e_of := coPset_elem_of_raw.
-Global Arguments coPset_elem_of_raw _ !_ / : simpl nomatch, assert.
-Lemma coPset_elem_of_node b l r p :
+Local Arguments coPset_elem_of_raw _ !_ / : simpl nomatch, assert.
+Local Lemma coPset_elem_of_node b l r p :
   e_of p (coPNode' b l r) = e_of p (coPNode b l r).
 Proof. by destruct p, b, l as [[]|], r as [[]|]. Qed.
 
 (** The full set and the empty set have a unique representation. *)
-Lemma coPLeaf_wf t b : (∀ p, e_of p t = b) → coPset_wf t → t = coPLeaf b.
+Local Lemma coPLeaf_wf t b : (∀ p, e_of p t = b) → coPset_wf t → t = coPLeaf b.
 Proof.
   induction t as [b'|b' l IHl r IHr]; intros Ht ?; [f_equal; apply (Ht 1)|].
   assert (b' = b) by (apply (Ht 1)); subst.
@@ -109,7 +111,7 @@ Proof.
 Qed.
 
 (** Equality is extensional. *)
-Lemma coPset_eq t1 t2 :
+Local Lemma coPset_eq t1 t2 :
   (∀ p, e_of p t1 = e_of p t2) → coPset_wf t1 → coPset_wf t2 → t1 = t2.
 Proof.
   revert t2.
@@ -123,7 +125,7 @@ Proof.
 Qed.
 
 (** Singleton. *)
-Fixpoint coPset_singleton_raw (p : positive) : coPset_raw :=
+Local Fixpoint coPset_singleton_raw (p : positive) : coPset_raw :=
   match p with
   | 1 => coPNode true (coPLeaf false) (coPLeaf false)
   | p~0 => coPNode' false (coPset_singleton_raw p) (coPLeaf false)
@@ -131,7 +133,7 @@ Fixpoint coPset_singleton_raw (p : positive) : coPset_raw :=
   end.
 
 (** Union. *)
-Global Instance coPset_union_raw : Union coPset_raw :=
+Local Instance coPset_union_raw : Union coPset_raw :=
   fix go t1 t2 := let _ : Union _ := @go in
   match t1, t2 with
   | coPLeaf false, coPLeaf false => coPLeaf false
@@ -144,7 +146,7 @@ Global Instance coPset_union_raw : Union coPset_raw :=
 Local Arguments union _ _!_ !_ / : assert.
 
 (** Intersection. *)
-Global Instance coPset_intersection_raw : Intersection coPset_raw :=
+Local Instance coPset_intersection_raw : Intersection coPset_raw :=
   fix go t1 t2 := let _ : Intersection _ := @go in
   match t1, t2 with
   | coPLeaf true, coPLeaf true => coPLeaf true
@@ -157,44 +159,47 @@ Global Instance coPset_intersection_raw : Intersection coPset_raw :=
 Local Arguments intersection _ _!_ !_ / : assert.
 
 (** Complement. *)
-Fixpoint coPset_opp_raw (t : coPset_raw) : coPset_raw :=
+Local Fixpoint coPset_opp_raw (t : coPset_raw) : coPset_raw :=
   match t with
   | coPLeaf b => coPLeaf (negb b)
   | coPNode b l r => coPNode' (negb b) (coPset_opp_raw l) (coPset_opp_raw r)
   end.
 
 (** Well-formedness for the above operations. *)
-Lemma coPset_singleton_wf p : coPset_wf (coPset_singleton_raw p).
+Local Lemma coPset_singleton_wf p : coPset_wf (coPset_singleton_raw p).
 Proof. induction p; simpl; eauto. Qed.
-Lemma coPset_union_wf t1 t2 : coPset_wf t1 → coPset_wf t2 → coPset_wf (t1 ∪ t2).
+Local Lemma coPset_union_wf t1 t2 :
+  coPset_wf t1 → coPset_wf t2 → coPset_wf (t1 ∪ t2).
 Proof. revert t2; induction t1 as [[]|[]]; intros [[]|[] ??]; simpl; eauto. Qed.
-Lemma coPset_intersection_wf t1 t2 :
+Local Lemma coPset_intersection_wf t1 t2 :
   coPset_wf t1 → coPset_wf t2 → coPset_wf (t1 ∩ t2).
 Proof. revert t2; induction t1 as [[]|[]]; intros [[]|[] ??]; simpl; eauto. Qed.
-Lemma coPset_opp_wf t : coPset_wf (coPset_opp_raw t).
+Local Lemma coPset_opp_wf t : coPset_wf (coPset_opp_raw t).
 Proof. induction t as [[]|[]]; simpl; eauto. Qed.
 
 (** Correctness for the above operations. *)
-Lemma coPset_elem_of_singleton p q : e_of p (coPset_singleton_raw q) ↔ p = q.
+Local Lemma coPset_elem_of_singleton p q :
+  e_of p (coPset_singleton_raw q) ↔ p = q.
 Proof.
   split; [|by intros <-; induction p; simpl; rewrite ?coPset_elem_of_node].
   by revert q; induction p; intros [?|?|]; simpl;
     rewrite ?coPset_elem_of_node; intros; f_equal/=; auto.
 Qed.
-Lemma coPset_elem_of_union t1 t2 p : e_of p (t1 ∪ t2) = e_of p t1 || e_of p t2.
+Local Lemma coPset_elem_of_union t1 t2 p :
+  e_of p (t1 ∪ t2) = e_of p t1 || e_of p t2.
 Proof.
   by revert t2 p; induction t1 as [[]|[]]; intros [[]|[] ??] [?|?|]; simpl;
     rewrite ?coPset_elem_of_node; simpl;
     rewrite ?orb_true_l, ?orb_false_l, ?orb_true_r, ?orb_false_r.
 Qed.
-Lemma coPset_elem_of_intersection t1 t2 p :
+Local Lemma coPset_elem_of_intersection t1 t2 p :
   e_of p (t1 ∩ t2) = e_of p t1 && e_of p t2.
 Proof.
   by revert t2 p; induction t1 as [[]|[]]; intros [[]|[] ??] [?|?|]; simpl;
     rewrite ?coPset_elem_of_node; simpl;
     rewrite ?andb_true_l, ?andb_false_l, ?andb_true_r, ?andb_false_r.
 Qed.
-Lemma coPset_elem_of_opp t p : e_of p (coPset_opp_raw t) = negb (e_of p t).
+Local Lemma coPset_elem_of_opp t p : e_of p (coPset_opp_raw t) = negb (e_of p t).
 Proof.
   by revert p; induction t as [[]|[]]; intros [?|?|]; simpl;
     rewrite ?coPset_elem_of_node; simpl.
@@ -267,18 +272,18 @@ Proof.
 Defined.
 
 (** * Finiteness *)
-(** The internal function [coPset_finite] determines whether
-    a (raw) set is finite. *)
+(** The internal function [coPset_finite] determines whether a (raw) set is
+finite. This definition is internal, use [set_finite] instead. *)
 Local Fixpoint coPset_finite (t : coPset_raw) : bool :=
   match t with
   | coPLeaf b => negb b | coPNode b l r => coPset_finite l && coPset_finite r
   end.
-Lemma coPset_finite_node b l r :
+Local Lemma coPset_finite_node b l r :
   coPset_finite (coPNode' b l r) = coPset_finite l && coPset_finite r.
 Proof. by destruct b, l as [[]|], r as [[]|]. Qed.
 (** This function is correct; it is equivalent to [set_finite], which is
     defined in terms of set membership. *)
-Lemma coPset_finite_spec X : set_finite X ↔ coPset_finite (`X).
+Local Lemma coPset_finite_spec X : set_finite X ↔ coPset_finite (`X).
 Proof.
   destruct X as [t Ht].
   unfold set_finite, elem_of at 1, coPset_elem_of; simpl; clear Ht; split.
@@ -304,10 +309,10 @@ Defined.
 (** * Picking an element out of an infinite set *)
 
 (** Provided that the set [X] is infinite, [coPpick X] yields an element of
-    this set. Note that [coPpick] is implemented by depth-first search, so
-    using it repeatedly to obtain elements [x] and inserting these elements
-    [x] into some set [Y] will give rise to a very unbalanced tree. *)
-Fixpoint coPpick_raw (t : coPset_raw) : option positive :=
+this set. Note that [coPpick] is implemented by depth-first search, so
+using it repeatedly to obtain elements [x] and inserting these elements
+[x] into some set [Y] will give rise to a very unbalanced tree. *)
+Local Fixpoint coPpick_raw (t : coPset_raw) : option positive :=
   match t with
   | coPLeaf true | coPNode true _ _ => Some 1
   | coPLeaf false => None
@@ -318,19 +323,19 @@ Fixpoint coPpick_raw (t : coPset_raw) : option positive :=
   end.
 Definition coPpick (X : coPset) : positive := default 1 (coPpick_raw (`X)).
 
-Lemma coPpick_raw_elem_of t i : coPpick_raw t = Some i → e_of i t.
+Local Lemma coPpick_raw_elem_of t i : coPpick_raw t = Some i → e_of i t.
 Proof.
   revert i; induction t as [[]|[] l ? r]; intros i ?; simplify_eq/=; auto.
   destruct (coPpick_raw l); simplify_option_eq; auto.
 Qed.
-Lemma coPpick_raw_None t : coPpick_raw t = None → coPset_finite t.
+Local Lemma coPpick_raw_None t : coPpick_raw t = None → coPset_finite t.
 Proof.
   induction t as [[]|[] l ? r]; intros i; simplify_eq/=; auto.
   destruct (coPpick_raw l); simplify_option_eq; auto.
 Qed.
 (** Provided [X] is infinite, the element [coPpick X] is a member of [X]. *)
 (** TODO: it should in fact be sufficient for [X] to be nonempty;
-    perhaps a stronger lemma can be proved in the future. *)
+perhaps a stronger lemma can be proved in the future. *)
 Lemma coPpick_elem_of X : ¬set_finite X → coPpick X ∈ X.
 Proof.
   destruct X as [t ?]; unfold coPpick; destruct (coPpick_raw _) as [j|] eqn:?.
@@ -374,13 +379,13 @@ Local Fixpoint Pset_ne_to_coPset_raw (t : Pmap_ne ()) : coPset_raw :=
 Local Definition Pset_to_coPset_raw : Pmap () → coPset_raw :=
   Pset_to_coPset_raw_aux Pset_ne_to_coPset_raw.
 
-Lemma Pset_to_coPset_raw_PNode ml mx mr :
+Local Lemma Pset_to_coPset_raw_PNode ml mx mr :
   pmap.PNode_valid ml mx mr →
   Pset_to_coPset_raw (pmap.PNode ml mx mr) =
     coPNode match mx with Some _ => true | None => false end
     (Pset_to_coPset_raw ml) (Pset_to_coPset_raw mr).
 Proof. by destruct ml, mx, mr. Qed.
-Lemma Pset_to_coPset_raw_wf t : coPset_wf (Pset_to_coPset_raw t).
+Local Lemma Pset_to_coPset_raw_wf t : coPset_wf (Pset_to_coPset_raw t).
 Proof.
   induction t as [|ml mx mr] using pmap.Pmap_ind; [done|].
   rewrite Pset_to_coPset_raw_PNode by done.
@@ -388,13 +393,14 @@ Proof.
     destruct mx; destruct ml using pmap.Pmap_ind; destruct mr using pmap.Pmap_ind;
     rewrite ?Pset_to_coPset_raw_PNode by done; naive_solver.
 Qed.
-Lemma elem_of_Pset_to_coPset_raw i t : e_of i (Pset_to_coPset_raw t) ↔ t !! i = Some ().
+Local Lemma elem_of_Pset_to_coPset_raw i t :
+  e_of i (Pset_to_coPset_raw t) ↔ t !! i = Some ().
 Proof.
   revert i. induction t as [|ml mx mr] using pmap.Pmap_ind; [done|].
   intros []; rewrite Pset_to_coPset_raw_PNode,
     pmap.Pmap_lookup_PNode by done; destruct mx as [[]|]; naive_solver.
 Qed.
-Lemma Pset_to_coPset_raw_finite t : coPset_finite (Pset_to_coPset_raw t).
+Local Lemma Pset_to_coPset_raw_finite t : coPset_finite (Pset_to_coPset_raw t).
 Proof.
   induction t as [|ml mx mr] using pmap.Pmap_ind; [done|].
   rewrite Pset_to_coPset_raw_PNode by done. destruct mx; naive_solver.
@@ -459,20 +465,19 @@ Proof.
 Defined.
 
 (** * Inverse suffix closure *)
-(** [coPset_suffixes q] is the set of all numbers [p] such that
-    [q] is a suffix of [p],
-    when these numbers are viewed as sequences of bits.
-    In other words, it is the set of all numbers
-    that have the suffix [q].
-    It is always an infinite set. *)
-Fixpoint coPset_suffixes_raw (p : positive) : coPset_raw :=
+(** [coPset_suffixes q] is the set of all numbers [p] such that [q] is a suffix
+of [p], when these numbers are viewed as sequences of bits. In other words, it
+is the set of all numbers that have the suffix [q]. It is always an infinite
+set. *)
+Local Fixpoint coPset_suffixes_raw (p : positive) : coPset_raw :=
   match p with
   | 1 => coPLeaf true
   | p~0 => coPNode' false (coPset_suffixes_raw p) (coPLeaf false)
   | p~1 => coPNode' false (coPLeaf false) (coPset_suffixes_raw p)
   end.
-Lemma coPset_suffixes_wf p : coPset_wf (coPset_suffixes_raw p).
+Local Lemma coPset_suffixes_wf p : coPset_wf (coPset_suffixes_raw p).
 Proof. induction p; simpl; eauto. Qed.
+
 Definition coPset_suffixes (p : positive) : coPset :=
   coPset_suffixes_raw p ↾ coPset_suffixes_wf _.
 Lemma elem_coPset_suffixes p q : p ∈ coPset_suffixes q ↔ ∃ q', p = q' ++ q.
@@ -489,24 +494,29 @@ Proof.
 Qed.
 
 (** * Splitting a set *)
-Fixpoint coPset_l_raw (t : coPset_raw) : coPset_raw :=
+(** Every infinite [X : coPset] can be split into two disjoint parts, which are
+infinite sets. In proofs, you typically want to use the lemmas [coPset_split]
+and [coPset_split_infinite]. Use the functions [coPset_l] and [coPset_r] if you
+need a constructive witness. *)
+Local Fixpoint coPset_l_raw (t : coPset_raw) : coPset_raw :=
   match t with
   | coPLeaf false => coPLeaf false
   | coPLeaf true => coPNode true (coPLeaf true) (coPLeaf false)
   | coPNode b l r => coPNode' b (coPset_l_raw l) (coPset_l_raw r)
   end.
-Fixpoint coPset_r_raw (t : coPset_raw) : coPset_raw :=
+Local Fixpoint coPset_r_raw (t : coPset_raw) : coPset_raw :=
   match t with
   | coPLeaf false => coPLeaf false
   | coPLeaf true => coPNode false (coPLeaf false) (coPLeaf true)
   | coPNode b l r => coPNode' false (coPset_r_raw l) (coPset_r_raw r)
   end.
 
-Lemma coPset_l_wf t : coPset_wf (coPset_l_raw t).
+Local Lemma coPset_l_wf t : coPset_wf (coPset_l_raw t).
 Proof. induction t as [[]|]; simpl; auto. Qed.
-Lemma coPset_r_wf t : coPset_wf (coPset_r_raw t).
+Local Lemma coPset_r_wf t : coPset_wf (coPset_r_raw t).
 Proof. induction t as [[]|]; simpl; auto. Qed.
-(** A set [X] can be split into two sets [coPset_l X] and [coPset_r X]. *)
+
+(* A set [X] can be split into two sets [coPset_l X] and [coPset_r X]. *)
 Definition coPset_l (X : coPset) : coPset :=
   let (t,Ht) := X in coPset_l_raw t ↾ coPset_l_wf _.
 Definition coPset_r (X : coPset) : coPset :=
@@ -549,7 +559,7 @@ Proof.
     coPset_lr_disjoint, coPset_l_finite, coPset_r_finite.
 Qed.
 (** Thus, in summary, every infinite set [X] can be split into two
-    disjoint parts, which are infinite sets. *)
+disjoint parts, which are infinite sets. *)
 Lemma coPset_split_infinite (X : coPset) :
   set_infinite X →
   ∃ X1 X2, X = X1 ∪ X2 ∧ X1 ∩ X2 = ∅ ∧ set_infinite X1 ∧ set_infinite X2.
